\section{Double-mode squeezing}

Let
\begin{equation}
\widehat{b}_i^-
= \frac{\widehat{a}_i^- - \beta \widehat{a}_j^+}{\sqrt{1-\vbr{\beta}^2}},\qquad
\widehat{b}_i^+ = \rbr{\widehat{b}_i^-}^\dagger
= \frac{\widehat{a}_i^+ - \beta^*\widehat{a}_j^-}{\sqrt{1-\vbr{\beta}^2}},
%\label{eq:res-bogolyubov-b}
\end{equation}
where $\cbr{i, j} = \cbr{1,2}$, so that
\begin{equation}
\sbr{\widehat{b}_i^-, \widehat{b}_j^+}_- =
\delta_{ij}\widehat{1}.
\end{equation}
One seeks the state $\Ket{\beta}$ satisfying
\begin{equation}
\widehat{b}^-\Ket{\beta} = 0.
%\label{eq:squeezed-state-def-1}
\end{equation}

Note that \cref{eq:res-bogolyubov-b} is again a restricted \emph{Bogolyubov
transformation}, in that the coefficients of $\widehat{a}_i^-$ for 
$\widehat{b}_i^-$ are real.

\subsection{Double-mode squeeze operator}
One attempts
\begin{equation}
\rfun{\widehat{S}_2}{z}\widehat{a}^-\rfun{\widehat{S_2}^{-1}}{z},
\end{equation}
where
\begin{equation}
\rfun{\widehat{S}_2}{z} \coloneqq \rfun{\exp}{z \widehat{a}_1^+ \widehat{a}_2^+ 
- z^*\widehat{a}_1^-\widehat{a}_2^-}
\end{equation}
is the \emph{double-mode squeeze operator}. Note that
\begin{equation}
\rfun{\widehat{S}_2^{-1}}{z} = \rfun{\widehat{S}_2}{-z}
= \rfun{\widehat{S}_2^\dagger}{z}.
\end{equation}

The parameterisation $z = r\ee^{\ii\phi}$ will also be used, where $r = 
\vbr{z}$, $\phi = \arg z$.

\begin{namedthm}{Proposition}
	%\label{nthm:prop-ad-aminus}
Let $X = z \widehat{a}_1^+ \widehat{a}_2^+ - z^*\widehat{a}_1^-\widehat{a}_2^-$. 
Then
\begin{align}
	\ad_X^{(2n)} \widehat{a}_i^- &= \vbr{z}^{2n} \widehat{a}_i^-
	= r^{2n} \widehat{a}_i^-,\\
	\ad_X^{(2n+1)} \widehat{a}_i^-
	&= -\vbr{z}^{2n+1}\frac{z}{\vbr{z}}\widehat{a}_j^+
	= \ee^{\ii\phi} r^{2n+1}\ee^{\ii\phi} \widehat{a}_j^+,
	\qquad \forall n \ge 0.
\end{align}
\end{namedthm} % Proposition

\begin{namedthm}{Proposition}
\begin{align}
	\rfun{\widehat{S}_2}{z} \widehat{a}_i^- \rfun{\widehat{S}_2^\dagger}{z}
	&= \widehat{a}_i^-\cosh \vbr{z}
		- \widehat{a}_j^+ \frac{z}{\vbr{z}} \sinh \vbr{z}
	\nonumber \\
	&= \widehat{a}_i^-\cosh r - \widehat{a}_j^+ \ee^{\ii\phi} \sinh r,
	%\label{eq:squeezed-aminus-parameter}
\end{align}
so that $z$ or $\rbr{r, \phi}$ is a parameterisation of $\beta$ in 
\cref{eq:res-bogolyubov-b} in that
\begin{equation}
	\vbr{\beta} = \tanh\vbr{z} = \tanh r,\qquad \arg \beta = \arg z = \phi.
	%\label{eq:beta-parameter}
\end{equation}
\end{namedthm} %Proposition

\begin{namedthm}{Squeezed ground state}
	$\Ket{\beta}$ in \cref{eq:squeezed-state-def-1} is the $\beta$-squeezed 
ground state, namely
\begin{equation}
	\Ket{\beta} = \rfun{\widehat{S}_2}{z}\Ket{0}.
\end{equation}
\end{namedthm} % Squeezed ground state



\subsection{Time evolution}

%\begin{namedthm}{Proposition}
%	Let $X = \ii\Omega t \rbr{a_1^+ a_1^- + a_2^+a_2^-}$, $Y = z a_1^+ a_2^+
%- z^* a_1^- a_2^-$.
%	\begin{equation}
%		\ad_X^{(n)}Y = z \rbr{+2\ii\Omega t}^n
%		\rbr{a^+}^2 - z^*\rbr{-2\ii\Omega t}^n\rbr{a^-}^2.
%	\end{equation}
%\end{namedthm} % Proposition

%\begin{namedthm}{Proposition}
%\begin{equation}
%\rfun{\mscrU}{t}\rfun{S}{z}	= \rfun{S}{z\ee^{2\ii\Omega t}}\rfun{\mscrU}{t}.
%\end{equation}
%\end{namedthm} % Proposition
%\begin{proof}
%Sum up.
%\end{proof}




\subsection{Particle numbers}

%\begin{equation}
%	\Braket{\beta | \widehat{a}^+\widehat{a}^- | \beta}
%	= \Braket{0 | \rfun{S^\dagger}{z}\widehat{a}^+
%	\widehat{a}^-\rfun{S}{z} | 0}
%	= \sinh^2 r = \frac{\vbr{\beta}^2}{1-\vbr{\beta}^2}.
%\end{equation}

%\begin{equation}
%	\Braket{0 | \widehat{b}^+\widehat{b}^- | 0}
%	= \Braket{0 | \rfun{S}{z}\widehat{a}^+\rfun{S^\dagger}{z}
%	\rfun{S}{z}\widehat{a}^-\rfun{S^\dagger}{z} | 0}
%	= \sinh^2 r = \frac{\vbr{\beta}^2}{1-\vbr{\beta}^2}.
%\end{equation}

\subsection{Wave function}

\begin{nameddef}{Wave function}
\begin{alignat}{3}
&\phantom{{}={}}&&\rbr{\frac{m\Omega}{2}}^{-1/2}\Braket{x_1, x_2 | \beta} 
\nonumber \\
&=&& \rbr{\cosh^2 r - \ee^{2\ii\phi} \sinh^2 r}^{-1/2} \nonumber \\
&&\cdot& \cfun{\exp}{-\frac{m\Omega}{2} \rbr{\frac{1 + \ee^{2\ii\phi}\tanh^2 r}%
{1 - \ee^{2\ii\phi}\tanh^2 r} \rbr{x_1^2+x_2^2} - \frac{4\ee^{\ii\phi}
\tanh r}{1 - \ee^{2\ii\phi}\tanh^2 r} x_1 x_2  }} \nonumber \\
&=&& \rbr{\frac{1-\vbr{\beta}^2}{1-\beta^2}}^{1/2}
\cfun{\exp}{-\frac{m\Omega}{2} \rbr{\frac{1+\beta^2}{1-\beta^2}\rbr{x_1^2+x_2^2}
- \frac{4\beta}{1-\beta^2} x_1 x_2}}.
\end{alignat}
\end{nameddef}

\subsection{Density matrix and Wigner function}

Did not find any simplification for $\Braket{x_1, x_2 | \widehat{\rho} | y_1,
y_2} \equiv \Braket{x_1, x_2 | \beta} \Braket{\beta | y_1,y_2} $.

\begin{alignat}{3}
&\phantom{{}={}}&&\rfun{W}{x_i; p_i} = \pp^{-2}
\exp\mathopen{}\left\{ -\rbr{
\frac{x_1^2+x_2^2}{\rbr{m\Omega}^{-1}}+
\frac{p_1^2+p_2^2}{\rbr{m\Omega}^{+1}}}\cosh 2r \mathclose{}\right.
\nonumber \\
&&+& \left.2\left(
 \rbr{\frac{x_1 x_2}{\rbr{m\Omega}^{-1}}
-\frac{p_1 p_2}{\rbr{m\Omega}^{+1}}} \cos\phi
-\rbr{x_1 p_2 + x_2 p_1} \sin\phi\right)\sinh 2r\right\}
\end{alignat}

Any insight?