\section{Notes on quantum mechanics}

\subsection{$\widehat{x}$ and $\widehat{p}$ acting on $\Ket{x}$}

\begin{namedthm}{Linear hermitian functions}
\begin{equation}
	\widehat{p} \Ket{x} = \rbr{+\ii \frpa{}{x}} \Ket{x},\qquad
	\Bra{x} \widehat{p} = \rbr{-\ii \frpa{}{x}} \Bra{x}.
\end{equation}

\end{namedthm} % Linear hermitian functions
\begin{proof}
\begin{align}
\Bra{x} \widehat{p} &= \int_{-\infty}^{+\infty}\dif p\,\Braket{x | p}
\Bra{p} \widehat{p} 
= \int_{-\infty}^{+\infty}\dif p\,\rbr{2\pp}^{-1/2}\ee^{\ii p x}
\Bra{p} p \nonumber \\
&= \int_{-\infty}^{+\infty}\dif p\,
\rbr{-\ii \frpa{}{x}} \rbr{2\pp}^{-1/2} \ee^{\ii p x} \Bra{p}
= \rbr{-\ii \frpa{}{x}} \int_{-\infty}^{+\infty}\dif p\,
\Braket{x | p} \Bra{p} \nonumber \\
&= \rbr{-\ii \frpa{}{x}} \Bra{x}.
\end{align}
\end{proof}

\begin{namedthm}{Linear unitary exponentials}

\begin{equation}
\ee^{\ii p_0 \widehat{x}} \Ket{x} = \ee^{\ii p_0 x} \Ket{x},
\qquad
\Bra{x} \ee^{\ii p_0 \widehat{x}} = \Bra{x} \ee^{\ii p_0 x};
\end{equation}
\begin{equation}
\ee^{\ii x_0 \widehat{p}} \Ket{x} = \Ket{x-x_0},\qquad
\Bra{x} \ee^{\ii x_0 \widehat{p}} = \Bra{x+x_0}.
\end{equation}

\end{namedthm} % Linear unitary exponentials

\begin{proof}
\begin{align}
\ee^{\ii x_0 \widehat{p}} \Ket{x} &= \int_{-\infty}^{+\infty} \dif p\,
\ee^{\ii x_0 \widehat{p}}\Ket{p}\Braket{p | x} \nonumber \\
&= \int_{-\infty}^{+\infty} \dif p\,
\ee^{\ii x_0 p}\Ket{p}\rbr{2\pp}^{-1/2}\ee^{-\ii x p}
= \int_{-\infty}^{+\infty} \dif p\,
\rbr{2\pp}^{-1/2}\ee^{-\ii \rbr{x-x_0} p}\Ket{p} \nonumber \\
&= \int_{-\infty}^{+\infty} \dif p\,
\Ket{p}\Braket{p | x-x_0} = \Ket{x-x_0};
\label{eq:displace-x-ket}
\end{align}

\begin{equation}
\Bra{x} \ee^{\ii x_0 \widehat{p}} = \int_{-\infty}^{+\infty} \dif p\,
\ee^{\ii x_0 p}\Bra{p}\rbr{2\pp}^{-1/2}\ee^{+\ii x p}
= \Bra{x+x_0}.
\label{eq:displace-x-bra}
\end{equation}

\end{proof}

\begin{namedthm}{Quadratic hermitian functions}
\begin{equation}
\widehat{x}^2 \Ket{x} = x^2 \Ket{x}, \qquad
\Bra{x} \widehat{x}^2 = \Bra{x} x^2;
\end{equation}
\begin{equation}
	\widehat{p}^2 \Ket{x} = -\frpa{^2}{x^2} \Ket{x}, \qquad
	\Bra{x} \widehat{p}^2 = -\frpa{^2}{x^2} \Bra{x};
\end{equation}
\begin{equation}
	\frac{\widehat{x}\widehat{p} + \widehat{p}\widehat{x}}{2} \Ket{x}
	= +\ii \rbr{\frac{1}{2}+x\frpa{}{x}} \Ket{x}, \qquad
	\Bra{x} \frac{\widehat{x}\widehat{p} + \widehat{p}\widehat{x}}{2}
	= -\ii \rbr{\frac{1}{2}+x\frpa{}{x}} \Bra{x}.
\end{equation}

\end{namedthm} % Quadratic hermitian functions
\begin{proof}
456
\end{proof}

\begin{namedthm}{Quadratic unitary exponentials}
\begin{equation}
\ee^{\ii \sigma \widehat{x}^2} \Ket{x} = \ee^{\ii \sigma x^2} \Ket{x},
\qquad
\Bra{x} \ee^{\ii \sigma \widehat{x}^2} = \Bra{x} \ee^{\ii \sigma x^2};
\end{equation}
\begin{align}
	\ee^{\ii \sigma \widehat{p}^2} \Ket{x}
	&= \rbr{-4\pp\ii\sigma}^{-1/2}\int_{-\infty}^{+\infty}\dif x'\,\Ket{x'}
	\cfun{\expi}{-\frac{\rbr{x-x'}^2}{4\sigma}}, \nonumber \\
	\Bra{x} \ee^{\ii \sigma \widehat{p}^2}
	&= \rbr{-4\pp\ii\sigma}^{-1/2}\int_{-\infty}^{+\infty}\dif x'\,\Bra{x'}
	\cfun{\expi}{-\frac{\rbr{x-x'}^2}{4\sigma}};
\end{align}
\begin{align}
	\ee^{\ii \lambda \rbr{\widehat{x}\widehat{p}
		+ \widehat{p}\widehat{x}}/2} \Ket{x}
	&= \ee^{-\lambda/2} \Ket{x\ee^{-\lambda}}, \nonumber \\
	\Bra{x} \ee^{\ii \lambda \rbr{\widehat{x}\widehat{p}
		+ \widehat{p}\widehat{x}}/2}
	&= \ee^{+\lambda/2} \bra{x\ee^{+\lambda}}.
\end{align}

\end{namedthm} % Quadratic unitary exponentials
\begin{proof}
789
\end{proof}



\subsection{Time evolution}

\begin{equation}
\rfun{\widehat{\mscrU}}{t;t_0} = \ee^{-\ii \widehat{H}\rbr{t-t_0}}
\end{equation}
is the time-evolution operator in the Schr√∂dinger picture.

\subsection{Wigner transformation}

\emph{Wigner transformation}
\begin{equation}
\rfun{g}{x,p} \coloneqq \frac{1}{2\pp}\int_{-\infty}^{+\infty}\dif s\,
\ee^{\ii p s} \Braket{ x-\frac{s}{2} | \widehat{G} | x + \frac{s}{2} }.
\end{equation}

\begin{equation}
\int_{\BbbR^2}\dif x\diff p\,\rfun{g}{x,p} \equiv \tr \widehat{G}.
\end{equation}

\